examples/tree_free.v
@@ -11,9 +11,17 @@ Inductive tree (x : ptr) (s : seq nat) (h : heap) : Prop :=
 | tree1 of x == 0 of
   perm_eq (s) (nil) /\ h = empty
 | tree2 of ~~ (x == 0) of
-  exists (v : nat) (s1 : seq nat) (s2 : seq nat) l r,
-  exists h_tree_ls1_523 h_tree_rs2_524,
-  perm_eq (s) ([:: v] ++ s1 ++ s2) /\ h = x :-> v \+ x .+ 1 :-> l \+ x .+ 2 :-> r \+ h_tree_ls1_523 \+ h_tree_rs2_524 /\ tree l s1 h_tree_ls1_523 /\ tree r s2 h_tree_rs2_524.
+  exists (v : nat) (s1 : seq nat) (s2 : seq nat) (l : ptr) (r : ptr),
+  exists h_tree_ls1_527 h_tree_rs2_528,
+  perm_eq (s) ([:: v] ++ s1 ++ s2) /\ h = x :-> v \+ x .+ 1 :-> l \+ x .+ 2 :-> r \+ h_tree_ls1_527 \+ h_tree_rs2_528 /\ tree l s1 h_tree_ls1_527 /\ tree r s2 h_tree_rs2_528.
+
+Inductive treeN (x : ptr) (n : nat) (h : heap) : Prop :=
+| treeN1 of x == 0 of
+  n == 0 /\ h = empty
+| treeN2 of ~~ (x == 0) of
+  exists (n1 : nat) (n2 : nat) (l : ptr) (r : ptr) (v : ptr),
+  exists h_treeN_ln1_529 h_treeN_rn2_530,
+  n == 1 + n1 + n2 /\ h = x :-> v \+ x .+ 1 :-> l \+ x .+ 2 :-> r \+ h_treeN_ln1_529 \+ h_treeN_rn2_530 /\ treeN l n1 h_treeN_ln1_529 /\ treeN r n2 h_treeN_rn2_530.
 
 Definition tree_free_type :=
   forall (vprogs : ptr),
@@ -22,8 +30,8 @@ Definition tree_free_type :=
     fun h =>
       let: (x) := vprogs in
       let: (s) := vghosts in
-      exists h_tree_xs_525,
-      h = h_tree_xs_525 /\ tree x s h_tree_xs_525,
+      exists h_tree_xs_531,
+      h = h_tree_xs_531 /\ tree x s h_tree_xs_531,
     [vfun (_: unit) h =>
       let: (x) := vprogs in
       let: (s) := vghosts in
@@ -42,54 +50,54 @@ Program Definition tree_free : tree_free_type :=
         tree_free (lx2);;
         tree_free (rx2);;
         dealloc x;;
-       dealloc (x .+ 1);;
-       dealloc (x .+ 2);;
+        dealloc (x .+ 1);;
+        dealloc (x .+ 2);;
         ret tt
     )).
 Obligation Tactic := intro; move=>x; ssl_program_simpl.
 Next Obligation.
 ssl_ghostelim_pre.
 move=>s.
-ex_elim h_tree_xs_525.
+ex_elim h_tree_xs_531.
 move=>[sigma_self].
 subst.
-move=>H_tree_xs_525.
+move=>H_tree_xs_531.
 ssl_ghostelim_post.
 ssl_open.
-ssl_open_post H_tree_xs_525.
-move=>[phi_tree_xs_525].
-move=>[sigma_tree_xs_525].
+ssl_open_post H_tree_xs_531.
+move=>[phi_tree_xs_531].
+move=>[sigma_tree_xs_531].
 subst.
 ssl_emp;
 sslauto.
-ssl_open_post H_tree_xs_525.
+ssl_open_post H_tree_xs_531.
 ex_elim vx2 s1x s2x lx2 rx2.
-ex_elim h_tree_lx2s1x_523x h_tree_rx2s2x_524x.
-move=>[phi_tree_xs_525].
-move=>[sigma_tree_xs_525].
+ex_elim h_tree_lx2s1x_527x h_tree_rx2s2x_528x.
+move=>[phi_tree_xs_531].
+move=>[sigma_tree_xs_531].
 subst.
-move=>[H_tree_lx2s1x_523x H_tree_rx2s2x_524x].
+move=>[H_tree_lx2s1x_527x H_tree_rx2s2x_528x].
 ssl_read.
 ssl_read.
-ssl_call_pre (h_tree_lx2s1x_523x).
+ssl_call_pre (h_tree_lx2s1x_527x).
 ssl_call (s1x).
-exists (h_tree_lx2s1x_523x);
+exists (h_tree_lx2s1x_527x);
 sslauto.
-move=>h_call5.
-move=>[sigma_call5].
+move=>h_call7.
+move=>[sigma_call7].
 subst.
 store_valid.
-ssl_call_pre (h_tree_rx2s2x_524x).
+ssl_call_pre (h_tree_rx2s2x_528x).
 ssl_call (s2x).
-exists (h_tree_rx2s2x_524x);
+exists (h_tree_rx2s2x_528x);
 sslauto.
-move=>h_call6.
-move=>[sigma_call6].
+move=>h_call8.
+move=>[sigma_call8].
 subst.
 store_valid.
-ssl_dealloc.
-ssl_dealloc.
-ssl_dealloc.
+ssl_dealloc (x).
+ssl_dealloc (x .+ 1).
+ssl_dealloc (x .+ 2).
 ssl_emp;
 sslauto.
 
