examples/tree_size.v
@@ -7,52 +7,21 @@ Require Import stmod stsep stlog stlogR.
 From SSL
 Require Import core.
 
-(*
-
-predicate treeN(loc x, int n) {
-|  x == 0        => { n == 0 ; emp }
-|  not (x == 0)  => { n == 1 + n1 + n2  /\  0 <= n1  /\  0 <= n2 ;
-  [x, 3] ** x :-> v ** (x + 1) :-> l ** (x + 2) :-> r ** treeN(l, n1) ** treeN(r, n2)}
-}
-
-
-{0 <= n ; r :-> 0 ** treeN(x, n)<a> }
-void tree_size(loc x, loc r)
-{true ; r :-> n ** treeN(x, n)<a> }
-
-#####
-
-void tree_size (loc x, loc r) {
-  if (x == 0) {
-  } else {
-    let l = *(x + 1);
-    let rx = *(x + 2);
-    tree_size(l, r);
-    let n1 = *r;
-    *r = 0;
-    tree_size(rx, r);
-    let n = *r;
-    *r = 1 + n1 + n;
-  }
-}
-
-*)
-
 Inductive tree (x : ptr) (s : seq nat) (h : heap) : Prop :=
 | tree1 of x == 0 of
   perm_eq (s) (nil) /\ h = empty
 | tree2 of ~~ (x == 0) of
-  exists (v : nat) (s1 : seq nat) (s2 : seq nat) l r,
-  exists h_tree_ls1_513 h_tree_rs2_514,
-  perm_eq (s) ([:: v] ++ s1 ++ s2) /\ h = x :-> v \+ x .+ 1 :-> l \+ x .+ 2 :-> r \+ h_tree_ls1_513 \+ h_tree_rs2_514 /\ tree l s1 h_tree_ls1_513 /\ tree r s2 h_tree_rs2_514.
+  exists (v : nat) (s1 : seq nat) (s2 : seq nat) (l : ptr) (r : ptr),
+  exists h_tree_ls1_519 h_tree_rs2_520,
+  perm_eq (s) ([:: v] ++ s1 ++ s2) /\ h = x :-> v \+ x .+ 1 :-> l \+ x .+ 2 :-> r \+ h_tree_ls1_519 \+ h_tree_rs2_520 /\ tree l s1 h_tree_ls1_519 /\ tree r s2 h_tree_rs2_520.
 
 Inductive treeN (x : ptr) (n : nat) (h : heap) : Prop :=
 | treeN1 of x == 0 of
   n == 0 /\ h = empty
 | treeN2 of ~~ (x == 0) of
-  exists n1 n2 l r (v: nat) (**),
-  exists h_treeN_ln1_515 h_treeN_rn2_516,
-  n == 1 + n1 + n2 /\ h = x :-> v \+ x .+ 1 :-> l \+ x .+ 2 :-> r \+ h_treeN_ln1_515 \+ h_treeN_rn2_516 /\ treeN l n1 h_treeN_ln1_515 /\ treeN r n2 h_treeN_rn2_516.
+  exists (n1 : nat) (n2 : nat) (l : ptr) (r : ptr) (v : ptr),
+  exists h_treeN_ln1_521 h_treeN_rn2_522,
+  n == 1 + n1 + n2 /\ h = x :-> v \+ x .+ 1 :-> l \+ x .+ 2 :-> r \+ h_treeN_ln1_521 \+ h_treeN_rn2_522 /\ treeN l n1 h_treeN_ln1_521 /\ treeN r n2 h_treeN_rn2_522.
 
 Definition tree_size_type :=
   forall (vprogs : ptr * ptr),
@@ -105,53 +74,51 @@ subst.
 ssl_emp;
 exists (empty);
 sslauto.
-(**)move/eqP in phi_treeN_xn_a.
-rewrite phi_treeN_xn_a=>//=.
+(**)move/eqP in phi_treeN_xn_a; subst=>//=.
 unfold_constructor 1;
 sslauto.
 ssl_open_post H_treeN_xn_a.
 ex_elim n1x2 n2x2 lx2 rx2 vx2.
-ex_elim h_treeN_lx2n1x2_515x h_treeN_rx2n2x2_516x.
+ex_elim h_treeN_lx2n1x2_521x h_treeN_rx2n2x2_522x.
 move=>[phi_treeN_xn_a].
 move=>[sigma_treeN_xn_a].
 subst.
-move=>[H_treeN_lx2n1x2_515x H_treeN_rx2n2x2_516x].
+move=>[H_treeN_lx2n1x2_521x H_treeN_rx2n2x2_522x].
 ssl_read.
 ssl_read.
-ssl_call_pre (r :-> 0 \+ h_treeN_lx2n1x2_515x).
+ssl_call_pre (r :-> 0 \+ h_treeN_lx2n1x2_521x).
 ssl_call (n1x2).
-exists (h_treeN_lx2n1x2_515x);
+exists (h_treeN_lx2n1x2_521x);
 sslauto.
-move=>h_call1.
-ex_elim h_treeN_lx2n1x2_515x.
-move=>[sigma_call1].
+move=>h_call3.
+ex_elim h_treeN_lx2n1x2_521x.
+move=>[sigma_call3].
 subst.
-move=>H_treeN_lx2n1x2_515x.
+move=>H_treeN_lx2n1x2_521x.
 store_valid.
 ssl_read.
 ssl_write r.
-ssl_call_pre (r :-> 0 \+ h_treeN_rx2n2x2_516x).
+ssl_call_pre (r :-> 0 \+ h_treeN_rx2n2x2_522x).
 ssl_call (n2x2).
-exists (h_treeN_rx2n2x2_516x);
+exists (h_treeN_rx2n2x2_522x);
 sslauto.
-move=>h_call2.
-ex_elim h_treeN_rx2n2x2_516x.
-move=>[sigma_call2].
+move=>h_call4.
+ex_elim h_treeN_rx2n2x2_522x.
+move=>[sigma_call4].
 subst.
-move=>H_treeN_rx2n2x2_516x.
+move=>H_treeN_rx2n2x2_522x.
 store_valid.
 ssl_read.
 ssl_write r.
 ssl_write_post r.
-(**)move/eqP in phi_treeN_xn_a.
-subst.
+(**)move/eqP in phi_treeN_xn_a; subst=>//=.
 ssl_emp;
-exists (x :-> vx2 \+ x .+ 1 :-> lx2 \+ x .+ 2 :-> rx2 \+ h_treeN_lx2n1x2_515x \+ h_treeN_rx2n2x2_516x).
-split.
-hhauto.
+exists (x :-> vx2 \+ x .+ 1 :-> lx2 \+ x .+ 2 :-> rx2 \+ h_treeN_lx2n1x2_521x \+ h_treeN_rx2n2x2_522x);
+sslauto.
 unfold_constructor 2;
 exists (n1x2), (n2x2), (lx2), (rx2), (vx2);
-exists (h_treeN_lx2n1x2_515x);
-exists (h_treeN_rx2n2x2_516x);
+exists (h_treeN_lx2n1x2_521x);
+exists (h_treeN_rx2n2x2_522x);
 sslauto.
+
 Qed.
