examples/dll_singleton.v
@@ -11,17 +11,17 @@ Inductive dll (x : ptr) (z : ptr) (s : seq nat) (h : heap) : Prop :=
 | dll1 of x == 0 of
   perm_eq (s) (nil) /\ h = empty
 | dll2 of ~~ (x == 0) of
-  exists (v : nat) (s1 : seq nat) w,
-  exists h_dll_wxs1_543,
-  perm_eq (s) ([:: v] ++ s1) /\ h = x :-> v \+ x .+ 1 :-> w \+ x .+ 2 :-> z \+ h_dll_wxs1_543 /\ dll w x s1 h_dll_wxs1_543.
+  exists (v : nat) (s1 : seq nat) (w : ptr),
+  exists h_dll_wxs1_549,
+  perm_eq (s) ([:: v] ++ s1) /\ h = x :-> v \+ x .+ 1 :-> w \+ x .+ 2 :-> z \+ h_dll_wxs1_549 /\ dll w x s1 h_dll_wxs1_549.
 
 Inductive sll (x : ptr) (s : seq nat) (h : heap) : Prop :=
 | sll1 of x == 0 of
   perm_eq (s) (nil) /\ h = empty
 | sll2 of ~~ (x == 0) of
-  exists (v : nat) (s1 : seq nat) nxt,
-  exists h_sll_nxts1_544,
-  perm_eq (s) ([:: v] ++ s1) /\ h = x :-> v \+ x .+ 1 :-> nxt \+ h_sll_nxts1_544 /\ sll nxt s1 h_sll_nxts1_544.
+  exists (v : nat) (s1 : seq nat) (nxt : ptr),
+  exists h_sll_nxts1_550,
+  perm_eq (s) ([:: v] ++ s1) /\ h = x :-> v \+ x .+ 1 :-> nxt \+ h_sll_nxts1_550 /\ sll nxt s1 h_sll_nxts1_550.
 
 Definition dll_singleton_type :=
   forall (vprogs : nat * ptr),
@@ -34,9 +34,9 @@ Definition dll_singleton_type :=
     [vfun (_: unit) h =>
       let: (x, r) := vprogs in
       let: (a) := vghosts in
-      exists (elems : seq nat) y,
-      exists h_dll_yelems_545,
-      perm_eq (elems) ([:: x]) /\ h = r :-> y \+ h_dll_yelems_545 /\ dll y 0 elems h_dll_yelems_545
+      exists elems y,
+      exists h_dll_yelems_551,
+      perm_eq (elems) ([:: x]) /\ h = r :-> y \+ h_dll_yelems_551 /\ dll y 0 elems h_dll_yelems_551
     ]).
 Program Definition dll_singleton : dll_singleton_type :=
   Fix (fun (dll_singleton : dll_singleton_type) vprogs =>
