examples/sll_append.v
@@ -1,5 +1,15 @@
 From mathcomp
-Require Import ssreflect ssrbool ssrnat eqtype seq ssrfun finset.
+Require Import ssreflect ssrbool ssrnat eqtype seq ssrfun.
+From fcsl
+Require Import prelude pred pcm unionmap heap.
+From HTT
+Require Import stmod stsep stlog stlogR.
+From SSL
+Require Import core.
+
+
+From mathcomp
+Require Import ssreflect ssrbool ssrnat eqtype seq ssrfun.
 From fcsl
 Require Import prelude pred pcm unionmap heap.
 From HTT
@@ -11,10 +21,11 @@ Inductive sll (x : ptr) (s : seq nat) (h : heap) : Prop :=
 | sll1 of x == 0 of
   perm_eq (s) (nil) /\ h = empty
 | sll2 of ~~ (x == 0) of
-  exists (v : nat) (s1 : seq nat) nxt,
-  exists h_sll528,
-    perm_eq s ([:: v] ++ s1) /\ h = x :-> v \+ x .+ 1 :-> nxt \+ h_sll528 /\ sll nxt s1 h_sll528.
+  exists (v : nat) (s1 : seq nat) (nxt : ptr),
+  exists h_sll_nxts1_513,
+  perm_eq (s) ([:: v] ++ s1) /\ h = x :-> v \+ x .+ 1 :-> nxt \+ h_sll_nxts1_513 /\ sll nxt s1 h_sll_nxts1_513.
 
+(* TODO: autogenerate *)
 Lemma sll_perm_eq x s h s1 :
   perm_eq s s1 -> sll x s h -> sll x s1 h.
 Proof.
@@ -30,7 +41,7 @@ sslauto.
 rewrite perm_sym in Heq.
 apply: (perm_trans Heq Heq1).
 Qed.
-
+(* end*)
 
 Definition sll_append_type :=
   forall (vprogs : ptr * ptr),
@@ -39,14 +50,14 @@ Definition sll_append_type :=
     fun h =>
       let: (x1, r) := vprogs in
       let: (s1, s2, x2) := vghosts in
-      exists h_sll529 h_sll530,
-      h = r :-> x2 \+ h_sll529 \+ h_sll530 /\ sll x1 s1 h_sll529 /\ sll x2 s2 h_sll530,
+      exists h_sll_x1s1_514 h_sll_x2s2_515,
+      h = r :-> x2 \+ h_sll_x1s1_514 \+ h_sll_x2s2_515 /\ sll x1 s1 h_sll_x1s1_514 /\ sll x2 s2 h_sll_x2s2_515,
     [vfun (_: unit) h =>
       let: (x1, r) := vprogs in
       let: (s1, s2, x2) := vghosts in
-      exists (s : seq nat) y,
-      exists h_sll531,
-      perm_eq s (s1 ++ s2) /\ h = r :-> y \+ h_sll531 /\ sll y s h_sll531
+      exists s y,
+      exists h_sll_ys_516,
+      perm_eq (s) (s1 ++ s2) /\ h = r :-> y \+ h_sll_ys_516 /\ sll y s h_sll_ys_516
     ]).
 Program Definition sll_append : sll_append_type :=
   Fix (fun (sll_append : sll_append_type) vprogs =>
@@ -67,40 +78,40 @@ Obligation Tactic := intro; move=>[x1 r]; ssl_program_simpl.
 Next Obligation.
 ssl_ghostelim_pre.
 move=>[[s1 s2] x22].
-move=>[h_sll529] [h_sll530].
+ex_elim h_sll_x1s1_514 h_sll_x22s2_515.
 move=>[sigma_self].
 subst.
-move=>[H_sll529 H_sll530].
+move=>[H_sll_x1s1_514 H_sll_x22s2_515].
 ssl_ghostelim_post.
 ssl_open.
-ssl_open_post H_sll529.
-move=>[phi_sll529].
-move=>[sigma_sll529].
+ssl_open_post H_sll_x1s1_514.
+move=>[phi_sll_x1s1_514].
+move=>[sigma_sll_x1s1_514].
 subst.
 ssl_emp;
 exists (nil ++ s2), (x22);
-exists (h_sll530);
+exists (h_sll_x22s2_515);
 sslauto.
-ssl_open_post H_sll529.
-move=>[vx12] [s1x1] [nxtx12].
-move=>[h_sll528x1].
-move=>[phi_sll529].
-move=>[sigma_sll529].
+ssl_open_post H_sll_x1s1_514.
+ex_elim vx12 s1x1 nxtx12.
+ex_elim h_sll_nxtx12s1x1_513x1.
+move=>[phi_sll_x1s1_514].
+move=>[sigma_sll_x1s1_514].
 subst.
-move=>H_sll528x1.
+move=>H_sll_nxtx12s1x1_513x1.
 ssl_read.
-ssl_call_pre (r :-> x22 \+ h_sll528x1 \+ h_sll530).
+ssl_call_pre (r :-> x22 \+ h_sll_nxtx12s1x1_513x1 \+ h_sll_x22s2_515).
 ssl_call (s1x1, s2, x22).
-exists (h_sll528x1);
-exists (h_sll530);
+exists (h_sll_nxtx12s1x1_513x1);
+exists (h_sll_x22s2_515);
 sslauto.
-move=>h_call8.
-move=>[s3] [y12].
-move=>[h_sll5311].
-move=>[phi_call8].
-move=>[sigma_call8].
+move=>h_call1.
+ex_elim s3 y12.
+ex_elim h_sll_y12s3_5161.
+move=>[phi_call1].
+move=>[sigma_call1].
 subst.
-move=>H_sll5311.
+move=>H_sll_y12s3_5161.
 store_valid.
 ssl_read.
 ssl_write (x1 .+ 1).
@@ -109,13 +120,12 @@ ssl_write r.
 ssl_write_post r.
 ssl_emp;
 exists ([:: vx12] ++ s1x1 ++ s2), (x1);
-exists (x1 :-> vx12 \+ x1 .+ 1 :-> y12 \+ h_sll5311);
+exists (x1 :-> vx12 \+ x1 .+ 1 :-> y12 \+ (*h_sll_y12s1x1s2_5161*) h_sll_y12s3_5161);
 sslauto.
-rewrite -cat_cons perm_cat2r perm_sym=>//=.
+(* *)rewrite -cat_cons perm_cat2r perm_sym=>//=.
 unfold_constructor 2;
 exists (vx12), (s1x1 ++ s2), (y12);
-exists (h_sll5311);
+exists (h_sll_y12s3_5161);
 sslauto.
 apply: (sll_perm_eq _ s3)=>//=.
 Qed.
-
