examples/sll_free.v
@@ -11,9 +11,9 @@ Inductive sll (x : ptr) (s : seq nat) (h : heap) : Prop :=
 | sll1 of x == 0 of
   perm_eq (s) (nil) /\ h = empty
 | sll2 of ~~ (x == 0) of
-  exists (v : nat) (s1 : seq nat) nxt,
-  exists h_sll_nxts1_529,
-  perm_eq (s) ([:: v] ++ s1) /\ h = x :-> v \+ x .+ 1 :-> nxt \+ h_sll_nxts1_529 /\ sll nxt s1 h_sll_nxts1_529.
+  exists (v : nat) (s1 : seq nat) (nxt : ptr),
+  exists h_sll_nxts1_535,
+  perm_eq (s) ([:: v] ++ s1) /\ h = x :-> v \+ x .+ 1 :-> nxt \+ h_sll_nxts1_535 /\ sll nxt s1 h_sll_nxts1_535.
 
 Definition sll_free_type :=
   forall (vprogs : ptr),
@@ -22,8 +22,8 @@ Definition sll_free_type :=
     fun h =>
       let: (x) := vprogs in
       let: (s) := vghosts in
-      exists h_sll_xs_530,
-      h = h_sll_xs_530 /\ sll x s h_sll_xs_530,
+      exists h_sll_xs_536,
+      h = h_sll_xs_536 /\ sll x s h_sll_xs_536,
     [vfun (_: unit) h =>
       let: (x) := vprogs in
       let: (s) := vghosts in
@@ -40,43 +40,43 @@ Program Definition sll_free : sll_free_type :=
         nxtx2 <-- @read ptr (x .+ 1);
         sll_free (nxtx2);;
         dealloc x;;
-       dealloc (x .+ 1);;
+        dealloc (x .+ 1);;
         ret tt
     )).
 Obligation Tactic := intro; move=>x; ssl_program_simpl.
 Next Obligation.
 ssl_ghostelim_pre.
 move=>s.
-ex_elim h_sll_xs_530.
+ex_elim h_sll_xs_536.
 move=>[sigma_self].
 subst.
-move=>H_sll_xs_530.
+move=>H_sll_xs_536.
 ssl_ghostelim_post.
 ssl_open.
-ssl_open_post H_sll_xs_530.
-move=>[phi_sll_xs_530].
-move=>[sigma_sll_xs_530].
+ssl_open_post H_sll_xs_536.
+move=>[phi_sll_xs_536].
+move=>[sigma_sll_xs_536].
 subst.
 ssl_emp;
 sslauto.
-ssl_open_post H_sll_xs_530.
+ssl_open_post H_sll_xs_536.
 ex_elim vx2 s1x nxtx2.
-ex_elim h_sll_nxtx2s1x_529x.
-move=>[phi_sll_xs_530].
-move=>[sigma_sll_xs_530].
+ex_elim h_sll_nxtx2s1x_535x.
+move=>[phi_sll_xs_536].
+move=>[sigma_sll_xs_536].
 subst.
-move=>H_sll_nxtx2s1x_529x.
+move=>H_sll_nxtx2s1x_535x.
 ssl_read.
-ssl_call_pre (h_sll_nxtx2s1x_529x).
+ssl_call_pre (h_sll_nxtx2s1x_535x).
 ssl_call (s1x).
-exists (h_sll_nxtx2s1x_529x);
+exists (h_sll_nxtx2s1x_535x);
 sslauto.
-move=>h_call8.
-move=>[sigma_call8].
+move=>h_call10.
+move=>[sigma_call10].
 subst.
 store_valid.
-ssl_dealloc.
-ssl_dealloc.
+ssl_dealloc (x).
+ssl_dealloc (x .+ 1).
 ssl_emp;
 sslauto.
 
