examples/sll_to_dll.v
@@ -1,0 +1,180 @@
+From mathcomp
+Require Import ssreflect ssrbool ssrnat eqtype seq ssrfun.
+From fcsl
+Require Import prelude pred pcm unionmap heap.
+From HTT
+Require Import stmod stsep stlog stlogR.
+From SSL
+Require Import core.
+
+Inductive dll (x : ptr) (z : ptr) (s : seq nat) (h : heap) : Prop :=
+| dll1 of x == 0 of
+  perm_eq (s) (nil) /\ h = empty
+| dll2 of ~~ (x == 0) of
+  exists (v : nat) (s1 : seq nat) w,
+  exists h_dll_wxs1_513,
+  perm_eq (s) ([:: v] ++ s1) /\ h = x :-> v \+ x .+ 1 :-> w \+ x .+ 2 :-> z \+ h_dll_wxs1_513 /\ dll w x s1 h_dll_wxs1_513.
+
+Inductive sll (x : ptr) (s : seq nat) (h : heap) : Prop :=
+| sll1 of x == 0 of
+  perm_eq (s) (nil) /\ h = empty
+| sll2 of ~~ (x == 0) of
+  exists (v : nat) (s1 : seq nat) nxt,
+  exists h_sll_nxts1_514,
+  perm_eq (s) ([:: v] ++ s1) /\ h = x :-> v \+ x .+ 1 :-> nxt \+ h_sll_nxts1_514 /\ sll nxt s1 h_sll_nxts1_514.
+
+Definition sll_to_dll_type :=
+  forall (vprogs : ptr),
+  {(vghosts : ptr * seq nat)},
+  STsep (
+    fun h =>
+      let: (f) := vprogs in
+      let: (x, s) := vghosts in
+      exists h_sll_xs_515,
+      h = f :-> x \+ h_sll_xs_515 /\ sll x s h_sll_xs_515,
+    [vfun (_: unit) h =>
+      let: (f) := vprogs in
+      let: (x, s) := vghosts in
+      exists i,
+      exists h_dll_is_516,
+      h = f :-> i \+ h_dll_is_516 /\ dll i 0 s h_dll_is_516
+    ]).
+Program Definition sll_to_dll : sll_to_dll_type :=
+  Fix (fun (sll_to_dll : sll_to_dll_type) vprogs =>
+    let: (f) := vprogs in
+    Do (
+      x2 <-- @read ptr f;
+      if x2 == 0
+      then
+        ret tt
+      else
+        vx22 <-- @read nat x2;
+        nxtx22 <-- @read ptr (x2 .+ 1);
+        f ::= nxtx22;;
+        sll_to_dll (f);;
+        i12 <-- @read ptr f;
+        if i12 == 0
+        then
+          i2 <-- allocb null 3;
+          dealloc x2;;
+          dealloc (x2 .+ 1);;
+          f ::= i2;;
+          (i2 .+ 1) ::= null;;
+          (i2 .+ 2) ::= null;;
+          i2 ::= vx22;;
+          ret tt
+        else
+          i2 <-- allocb null 3;
+          dealloc x2;;
+          dealloc (x2 .+ 1);;
+          (i12 .+ 2) ::= i2;;
+          f ::= i2;;
+          (i2 .+ 1) ::= i12;;
+          (i2 .+ 2) ::= null;;
+          i2 ::= vx22;;
+          ret tt
+    )).
+Obligation Tactic := intro; move=>f; ssl_program_simpl.
+Next Obligation.
+ssl_ghostelim_pre.
+move=>[x2 s].
+ex_elim h_sll_x2s_515.
+move=>[sigma_self].
+subst.
+move=>H_sll_x2s_515.
+ssl_ghostelim_post.
+ssl_read.
+ssl_open.
+ssl_open_post H_sll_x2s_515.
+move=>[phi_sll_x2s_515].
+move=>[sigma_sll_x2s_515].
+subst.
+ssl_emp;
+exists (0);
+exists (empty);
+sslauto.
+unfold_constructor 1;
+sslauto.
+ssl_open_post H_sll_x2s_515.
+ex_elim vx22 s1x2 nxtx22.
+ex_elim h_sll_nxtx22s1x2_514x2.
+move=>[phi_sll_x2s_515].
+move=>[sigma_sll_x2s_515].
+subst.
+move=>H_sll_nxtx22s1x2_514x2.
+ssl_read.
+ssl_read.
+ssl_write f.
+ssl_call_pre (f :-> nxtx22 \+ h_sll_nxtx22s1x2_514x2).
+ssl_call (nxtx22, s1x2).
+exists (h_sll_nxtx22s1x2_514x2);
+sslauto.
+move=>h_call1.
+ex_elim i12.
+ex_elim h_dll_i12s1x2_5161.
+move=>[sigma_call1].
+subst.
+move=>H_dll_i12s1x2_5161.
+store_valid.
+ssl_read.
+ssl_open.
+ssl_open_post H_dll_i12s1x2_5161.
+move=>[phi_dll_i12s1x2_5161].
+move=>[sigma_dll_i12s1x2_5161].
+subst.
+ssl_alloc i2.
+ssl_dealloc x2.
+ssl_dealloc (x2 .+ 1).
+ssl_write f.
+ssl_write_post f.
+ssl_write (i2 .+ 1).
+ssl_write_post (i2 .+ 1).
+ssl_write (i2 .+ 2).
+ssl_write_post (i2 .+ 2).
+ssl_write i2.
+ssl_write_post i2.
+ssl_emp;
+exists (i2);
+exists (i2 :-> vx22 \+ i2 .+ 1 :-> null \+ i2 .+ 2 :-> null);
+sslauto.
+unfold_constructor 2;
+exists (vx22), (nil), (0);
+exists (empty);
+sslauto.
+unfold_constructor 1;
+sslauto.
+ssl_open_post H_dll_i12s1x2_5161.
+ex_elim vi122 s1i12 wi122.
+ex_elim h_dll_wi122i12s1i12_513i12.
+move=>[phi_dll_i12s1x2_5161].
+move=>[sigma_dll_i12s1x2_5161].
+subst.
+move=>H_dll_wi122i12s1i12_513i12.
+ssl_alloc i2.
+ssl_dealloc x2.
+ssl_dealloc (x2 .+ 1).
+ssl_write (i12 .+ 2).
+ssl_write_post (i12 .+ 2).
+ssl_write f.
+ssl_write_post f.
+ssl_write (i2 .+ 1).
+ssl_write_post (i2 .+ 1).
+ssl_write (i2 .+ 2).
+ssl_write_post (i2 .+ 2).
+ssl_write i2.
+ssl_write_post i2.
+ssl_emp;
+exists (i2);
+exists (i2 :-> vx22 \+ i2 .+ 1 :-> i12 \+ i2 .+ 2 :-> null \+ i12 :-> vi122 \+ i12 .+ 1 :-> wi122 \+ i12 .+ 2 :-> i2 \+ h_dll_wi122i12s1i12_513i12);
+sslauto.
+unfold_constructor 2;
+exists (vx22), ([:: vi122] ++ s1i12), (i12);
+exists (i12 :-> vi122 \+ i12 .+ 1 :-> wi122 \+ i12 .+ 2 :-> i2 \+ h_dll_wi122i12s1i12_513i12);
+sslauto.
+(**)admit.
+unfold_constructor 2;
+exists (vi122), (s1i12), (wi122);
+exists (h_dll_wi122i12s1i12_513i12);
+sslauto.
+
+Qed.
